Progress with for/par result.
Move some things around to keep them tidy.

Also now believe I have a good characterisation of the correctness
condition required of the wave array.

Substitutions and variable names are a slight issue: the statement of
correctness now includes assumptions stating that new variable names
have to be suitably fresh.

hol/pc-verification/forparConvertScript.sml
@@ -8,8 +8,12 @@ open PseudoCOpsTheory
 open PseudoCPropsTheory
 open hidagTheory
 open PseudoCHDAGTheory
+open monadsyntax boolSimps
+open lcsymtacs
 
 val _ = new_theory "forparConvert";
+
+val _ = set_trace "Goalstack.print_goal_at_top" 0
 
 (* for compatibility with old PC syntax *)
 val _ = temp_overload_on ("ARead", ``λs e. MAccess (ASub (VRead s) e)``)
@@ -30,26 +34,69 @@ But will first aim for the simpler (less realistic):
 
     for (w ∈ 0 .. wavedepth g) {
       parfor (i ∈ d) {
-        if (wave[i] == w) { body }
+        if (wave_a[i] == w) { body }
       }
     }
 
-where the wave array maps iteration numbers to wave number.
+where the wave_a array maps iteration numbers to wave number, which notion is captured by the wave_array_correct relation.
 
 *)
+val wave_array_correct_def = Define`
+  wave_array_correct anm lo hi graph mem ⇔
+    lo ≤ hi ∧
+    ∃avalue.
+      FLOOKUP mem anm = SOME (Array avalue) ∧
+      LENGTH avalue = Num (hi - lo) ∧
+      ∀i wnum. lo ≤ i ∧ i < hi ⇒
+               (EL (Num (i - lo)) avalue = Int wnum ⇔
+                0 ≤ wnum ∧
+                ∃sg. HG sg <: wave (Num wnum) graph ∧
+                     ∀n. n <: allnodes sg ⇒ [Int i] <<= FST n.data)
+`;
+
+val strip_purereads_IDEM = store_thm(
+  "strip_purereads_IDEM",
+  ``strip_purereads (strip_purereads g) = strip_purereads g``,
+  simp[gafilter_gafilter, combinTheory.o_DEF]);
+
+(*
+val graphOf_ForLoop_Seq = store_thm(
+  "graphOf_ForLoop_Seq",
+  ``graphOf lab m (ForLoop i (D lo hi) body) =
+      case (evalexpr m lo, evalexpr m hi) of
+        (Int lo_i, Int hi_i) => if lo_i <= hi_i then
+*)
+
+val domreadAction_write = store_thm(
+  "domreadAction_write[simp]",
+  ``(domreadAction l m d).write = NONE``,
+  Cases_on `d` >> simp[domreadAction_def]);
+
 val simple_executor_equivalence = store_thm(
   "simple_executor_equivalence",
-  ``graphOf lab0 m0 (ForLoop i d body) = SOME(m,g) ⇒
+  ``evalexpr m0 lo = Int loi ∧
+    evalexpr m0 hi = Int hii ∧
+    wave_array_correct wave_a loi hii g m0 ∧
+    w ≠ i ∧ wave_a ≠ i ∧ wave_a ≠ w ∧ w # lo ∧ w # hi ∧
+    graphOf [] m0 (ForLoop i (D lo hi) body) = SOME(m,g) ⇒
     ∃g'.
-      graphOf lab0 m0
+      graphOf [] m0
         (ForLoop
            w
            (D (Value (Int 0)) (Value (Int &(wavedepth g))))
-           (ParLoop i d
+           (ParLoop i (D lo hi)
               (IfStmt (ARead wave_a (VarExpr i) == VarExpr w)
                       body
                       Done))) = SOME(m,g') ∧
-      strip_pure_reads g' = g``,
-  NO_TAC);
+      strip_purereads g' = g``,
+  ONCE_REWRITE_TAC [graphOf_def] >>
+  csimp[dvalues_def, evalexpr_def, PULL_EXISTS, EXISTS_PROD,
+        FORALL_PROD, ssubst_def, esubst_def] >>
+  simp[rich_listTheory.FOLDL_FOLDR_REVERSE, MAP_GENLIST,
+       REVERSE_GENLIST, combinTheory.o_ABS_R,
+       DECIDE ``PRE n - m = n - (m + 1)``] >>
+  qx_gen_tac `g0` >> strip_tac >>
+  `loi ≤ hii` by fs[wave_array_correct_def] >> fs[]
+ );
 
 val _ = export_theory();
